src/PermInstr.v
@@ -51,14 +51,14 @@ Qed.
 
 Hint Resolve HS_nil.
 
-Definition false_pred {AT AEQ V} (m: @mem AT AEQ V) := False.
+Definition false_pred {AT AEQ V}:= lift_empty(False)(AT:=AT)(AEQ:=AEQ)(V:=V).
 Hint Unfold false_pred.
 
 Lemma false_pred_all:
   forall AT AEQ V (P: @pred AT AEQ V),
     false_pred =p=> P.
 Proof.
-  unfold pimpl; simpl; intuition.
+  unfold false_pred; intros; cancel.
 Qed.
 
 Hint Resolve false_pred_all.
@@ -344,7 +344,48 @@ Theorem hash_ok:
     false_pred (* Can't crash *)                            
   >!} Hash buf.
 Proof.
-Admitted.
+  unfold corr2; intros.
+  destruct_lift H; cleanup.
+  repeat inv_exec_perm; simpl in *; cleanup.
+  {
+    edestruct H4; eauto.
+    pred_apply; cancel; eauto.
+    solve_hashmap_subset.
+    split; auto.
+    clear H0; eapply bind_secure; intuition.  
+    unfold permission_secure; intros.
+    inv_exec_perm; cleanup; auto.
+    simpl; eauto.
+    simpl; eauto.
+    
+    unfold permission_secure; intros.
+    clear H1.
+    inv_exec_perm; cleanup; auto.
+    edestruct H4; eauto.
+    pred_apply; cancel; eauto.
+    solve_hashmap_subset.
+  }
+  split_ors; cleanup; inv_exec_perm.
+  {
+    split.
+    right; do 3 eexists; intuition.
+    edestruct H4; eauto; cleanup.
+    pred_apply; cancel; eauto.
+    solve_hashmap_subset.
+    split_ors; cleanup; try congruence.
+    eapply bind_secure; intuition.
+    unfold permission_secure; intros.
+    inv_exec_perm; cleanup; auto.
+    simpl; eauto.
+    simpl; eauto.
+    unfold permission_secure; intros.
+    inv_exec_perm; cleanup; auto.
+    edestruct H4; eauto.
+    pred_apply; cancel; eauto.
+    solve_hashmap_subset.
+  }
+Qed.
+
 
 Theorem hash2_ok:
   forall sz1 sz2 (buf1 : word sz1) (buf2 : word sz2) pr,
@@ -361,7 +402,161 @@ Theorem hash2_ok:
     false_pred (* Can't crash *)           
   >!} Hash2 buf1 buf2.
 Proof.
-Admitted.
+  unfold corr2; intros.
+  destruct_lift H; cleanup.
+  repeat inv_exec_perm; simpl in *; cleanup.
+  {
+    edestruct H4; eauto.
+    pred_apply; cancel; eauto.
+    solve_hashmap_subset.
+    split; auto.
+    clear H0; eapply bind_secure; intuition.  
+    unfold permission_secure; intros.
+    inv_exec_perm; cleanup; auto.
+    simpl; eauto.
+    simpl; eauto.
+    
+    unfold permission_secure; intros.
+    clear H1.
+    inv_exec_perm; cleanup; auto.
+    edestruct H4; eauto.
+    pred_apply; cancel; eauto.
+    solve_hashmap_subset.
+  }
+  split_ors; cleanup; inv_exec_perm.
+  {
+    split.
+    right; do 3 eexists; intuition.
+    edestruct H4; eauto; cleanup.
+    pred_apply; cancel; eauto.
+    solve_hashmap_subset.
+    split_ors; cleanup; try congruence.
+    eapply bind_secure; intuition.
+    unfold permission_secure; intros.
+    inv_exec_perm; cleanup; auto.
+    simpl; eauto.
+    simpl; eauto.
+    unfold permission_secure; intros.
+    inv_exec_perm; cleanup; auto.
+    edestruct H4; eauto.
+    pred_apply; cancel; eauto.
+    solve_hashmap_subset.
+  }
+Qed.
+
+Theorem hashhandle_ok:
+  forall i pr,
+  {!< F tb,
+  PERM: pr
+  PRE:bm, hm,
+    F * [[ bm i = Some tb ]]
+  POST:bm', hm',
+    RET:h     F * [[ bm' = bm ]] *
+              [[ hash_safe hm h (encode tb) ]] *
+              [[ h = hash_fwd (encode tb) ]] *
+              [[ hm' = upd_hashmap' hm h (encode tb) ]]
+  CRASH:bm'', hm'',
+    false_pred (* Can't crash *)           
+  >!} HashHandle i.
+Proof.
+  unfold corr2; intros.
+  destruct_lift H; cleanup.
+  repeat inv_exec_perm; simpl in *; cleanup.
+  {
+    edestruct H4; eauto.
+    pred_apply; cancel; eauto.
+    solve_hashmap_subset.
+    split; auto.
+    clear H0; eapply bind_secure; intuition.  
+    unfold permission_secure; intros.
+    inv_exec_perm; cleanup; auto.
+    simpl; eauto.
+    simpl; eauto.
+    
+    unfold permission_secure; intros.
+    clear H1.
+    inv_exec_perm; cleanup; auto.
+    edestruct H4; eauto.
+    pred_apply; cancel; eauto.
+    solve_hashmap_subset.
+  }
+  split_ors; cleanup; inv_exec_perm.
+  {
+    split.
+    right; do 3 eexists; intuition.
+    edestruct H4; eauto; cleanup.
+    pred_apply; cancel; eauto.
+    solve_hashmap_subset.
+    split_ors; cleanup; try congruence.
+    eapply bind_secure; intuition.
+    unfold permission_secure; intros.
+    inv_exec_perm; cleanup; auto.
+    simpl; eauto.
+    simpl; eauto.
+    unfold permission_secure; intros.
+    inv_exec_perm; cleanup; auto.
+    edestruct H4; eauto.
+    pred_apply; cancel; eauto.
+    solve_hashmap_subset.
+  }
+Qed.
+
+Theorem hashhandle2_ok:
+  forall sz (buf2 : word sz) i pr,
+  {!< F tb,
+  PERM: pr
+  PRE:bm, hm,
+    F * [[ bm i = Some tb ]]
+  POST:bm', hm',
+    RET:h     F * [[ bm' = bm ]] *
+              [[ hash_safe hm h (Word.combine (encode tb) buf2) ]] *
+              [[ h = hash_fwd (Word.combine (encode tb) buf2) ]] *
+              [[ hm' = upd_hashmap' hm h (Word.combine (encode tb) buf2) ]]
+  CRASH:bm'', hm'',
+    false_pred (* Can't crash *)           
+  >!} HashHandle2 i buf2.
+Proof.
+  unfold corr2; intros.
+  destruct_lift H; cleanup.
+  repeat inv_exec_perm; simpl in *; cleanup.
+  {
+    edestruct H4; eauto.
+    pred_apply; cancel; eauto.
+    solve_hashmap_subset.
+    split; auto.
+    clear H0; eapply bind_secure; intuition.  
+    unfold permission_secure; intros.
+    inv_exec_perm; cleanup; auto.
+    simpl; eauto.
+    simpl; eauto.
+    
+    unfold permission_secure; intros.
+    clear H1.
+    inv_exec_perm; cleanup; auto.
+    edestruct H4; eauto.
+    pred_apply; cancel; eauto.
+    solve_hashmap_subset.
+  }
+  split_ors; cleanup; inv_exec_perm.
+  {
+    split.
+    right; do 3 eexists; intuition.
+    edestruct H4; eauto; cleanup.
+    pred_apply; cancel; eauto.
+    solve_hashmap_subset.
+    split_ors; cleanup; try congruence.
+    eapply bind_secure; intuition.
+    unfold permission_secure; intros.
+    inv_exec_perm; cleanup; auto.
+    simpl; eauto.
+    simpl; eauto.
+    unfold permission_secure; intros.
+    inv_exec_perm; cleanup; auto.
+    edestruct H4; eauto.
+    pred_apply; cancel; eauto.
+    solve_hashmap_subset.
+  }
+Qed.
 
 Lemma ret_secure:
   forall T pr (v: T),
@@ -636,6 +831,8 @@ Hint Extern 1 (corr2 _ _ (Bind (Seal _ _) _)) => apply seal_secure : prog.
 Hint Extern 1 (corr2 _ _ (Bind (Unseal _) _)) => apply unseal_secure : prog.
 Hint Extern 1 ({{_|_}} Bind (Hash _) _) => apply hash_ok : prog.
 Hint Extern 1 ({{_|_}} Bind (Hash2 _ _) _) => apply hash2_ok : prog.
+Hint Extern 1 ({{_|_}} Bind (HashHandle _) _) => apply hashhandle_ok : prog.
+Hint Extern 1 ({{_|_}} Bind (HashHandle2 _ _) _) => apply hashhandle2_ok : prog.
 Hint Extern 1 (corr2 _ _ (Bind Sync _)) => apply sync_secure : prog.
 Hint Extern 1 (corr2 _ _ (Bind (Ret _) _)) => apply ret_secure : prog.
 
