src/PermRecArrayUtils.v
@@ -1091,5 +1091,5 @@ Lemma synced_list_ipack_length_ok : forall len i items,
     erewrite Rec.word_updN'_equiv by auto.
     reflexivity.
   Qed.
-
+    
 End RADefs.
